src/dvspec/dafny/att_spec_proofs/incomplete_proofs.dfy
@@ -25,30 +25,104 @@ module Incomplete_Proofs
     import opened DVN_Next_Invs_8_18
     import opened Fnc_Inv    
 
-    lemma {:axiom} axiom_inv18(dvc: DVCNodeState)    
-    ensures inv18_body(dvc)
+    lemma {:axiom} axiom_inv19(dvc: DVCNodeState)    
+    ensures inv19_body(dvc)
 
     
+
      
     
+    
+
+    
+
+    lemma lemma_inv19_f_check_for_next_queued_duty(
+        process: DVCNodeState,
+        process': DVCNodeState
+    )
+    requires f_check_for_next_queued_duty.requires(process)
+    requires process' == f_check_for_next_queued_duty(process).state        
+    requires inv19_body(process)    
+    // ensures inv19_body(process')
+    decreases process.attestation_duties_queue
+    {
+        if  && process.attestation_duties_queue != [] 
+            && (
+                || process.attestation_duties_queue[0].slot in process.future_att_consensus_instances_already_decided
+                || !process.current_attestation_duty.isPresent()
+            )    
+        {            
+                if process.attestation_duties_queue[0].slot in process.future_att_consensus_instances_already_decided.Keys 
+                {
+                    var queue_head := process.attestation_duties_queue[0];
+                    var new_attestation_slashing_db := f_update_attestation_slashing_db(process.attestation_slashing_db, process.future_att_consensus_instances_already_decided[queue_head.slot]);
+                    var process_mod := process.(
+                        attestation_duties_queue := process.attestation_duties_queue[1..],
+                        future_att_consensus_instances_already_decided := process.future_att_consensus_instances_already_decided - {queue_head.slot},
+                        attestation_slashing_db := new_attestation_slashing_db,
+                        attestation_consensus_engine_state := updateConsensusInstanceValidityCheck(
+                            process.attestation_consensus_engine_state,
+                            new_attestation_slashing_db
+                        )                        
+                    );
+                    assert inv9_body(process_mod);
+                    lemma_inv19_f_check_for_next_queued_duty(process_mod, process');
+                }
+                else
+                { 
+                    var next_duty := process.attestation_duties_queue[0];
+                    var process_mod := process.(
+                        attestation_duties_queue := process.attestation_duties_queue[1..]
+                    );     
+
+                    assert forall queued_duty: AttestationDuty | 
+                                queued_duty in process_mod.attestation_duties_queue ::
+                                    next_duty.slot <= queued_duty.slot;
+
+                    assert inv19_body(process_mod);
+                    lemma_inv19_f_start_next_duty(process_mod, next_duty, process');
+                }
+        }
+        else
+        {  }
+    }
+
+    lemma lemma_inv19_f_serve_attestation_duty(
+        process: DVCNodeState,
+        attestation_duty: AttestationDuty,
+        process': DVCNodeState
+    )  
+    requires f_serve_attestation_duty.requires(process, attestation_duty)
+    requires process' == f_serve_attestation_duty(process, attestation_duty).state
+    requires inv19_body(process)
+    ensures inv19_body(process')
+    {
+        var process_mod := process.(
+                attestation_duties_queue := process.attestation_duties_queue + [attestation_duty],
+                all_rcvd_duties := process.all_rcvd_duties + {attestation_duty}
+            );  
+
+        if process.latest_attestation_duty.isPresent() 
+        {
+            assert process_mod.latest_attestation_duty.isPresent();
+            assert process.latest_attestation_duty.safe_get()
+                        == process_mod.latest_attestation_duty.safe_get();
+            assert process.latest_attestation_duty.safe_get().slot <= attestation_duty.slot;
+            assert process_mod.latest_attestation_duty.safe_get().slot <= attestation_duty.slot;            
+            assert inv19_body(process_mod);      
+        }
+        else 
+        {
+            assert !process_mod.latest_attestation_duty.isPresent();              
+            assert inv19_body(process_mod);      
+        }
+        
+        lemma_inv19_f_check_for_next_queued_duty(process_mod, process');        
+    } 
+
+    
 
      
-
-    
-
-    
-
-    
-    
-
-    
-
-    
-
-    
-    
-
-    
-      
-    
+     
+       
 }
